substitution and inversion lemmas

logic.lean
@@ -2,125 +2,287 @@ import .syntax .etc .props
 
 -- instantiation
 
-constant prop.instantiated: prop → qfprop → Prop
+constant prop.instantiated_p: prop → qfprop
+
+constant prop.instantiated_n: prop → qfprop
+
+def prop.erased_p: prop → qfprop := sorry
+
+def prop.erased_n: prop → qfprop := sorry
 
 -- substitution
 
-inductive term.substituted (x: var) (v: value): term → term → Prop
+def term.subst (x: var) (v: value): term → term
+| (term.value v')       := v'
+| (term.var y)          := if x = y then v else y
+| (term.unop op t)      := term.unop op t.subst
+| (term.binop op t₁ t₂) := term.binop op t₁.subst t₂.subst
+| (term.app t₁ t₂)      := term.app t₁.subst t₂.subst
 
-| value {v': value} :
-    term.substituted v' v'
+def spec.subst (x: var) (v: value): spec → spec
+| (spec.term t) :=
+    spec.term (term.subst x v t)
+| (spec.not R) :=
+    have R.size < R.not.size, from lt_of_add_one,
+    spec.not R.subst
+| (spec.and R S) :=
+    have R.size < (R & S).size, from lt_of_add.left,
+    have S.size < (R & S).size, from lt_of_add.right,
+    R.subst & S.subst
+| (spec.or R S) :=
+    have R.size < (R & S).size, from lt_of_add.left,
+    have S.size < (R & S).size, from lt_of_add.right,
+    spec.or R.subst S.subst
+| (spec.func t y R S) :=
+    have R.size < (R & S).size, from lt_of_add.left,
+    have S.size < (R & S).size, from lt_of_add.right,
+    if x = y
+    then spec.func (term.subst x v t) x R S
+    else spec.func (term.subst x v t) y R.subst S.subst
 
-| same_var:
-    term.substituted x v
+def spec.subst_env: env → spec → spec
+| env.empty R := R
+| (σ[x↦v]) R :=
+    have σ.size < (σ[x ↦ v].size), from lt_of_add_one,
+    spec.subst x v (spec.subst_env σ R)
 
-| diff_var {y: var}:
-    (x ≠ y) →
-    term.substituted y y
+def qfprop.subst (x: var) (v: value): qfprop → qfprop
+| (qfprop.term t)        := term.subst x v t
+| (qfprop.not P)         := qfprop.not P.subst
+| (qfprop.and P Q)       := P.subst & Q.subst
+| (qfprop.or P Q)        := qfprop.or P.subst Q.subst
+| (qfprop.pre t₁ t₂)     := qfprop.pre (term.subst x v t₁) (term.subst x v t₂)
+| (qfprop.pre₁ op t)     := qfprop.pre₁ op (term.subst x v t)
+| (qfprop.pre₂ op t₁ t₂) := qfprop.pre₂ op (term.subst x v t₁) (term.subst x v t₂)
+| (qfprop.post t₁ t₂)    := qfprop.post (term.subst x v t₁) (term.subst x v t₂)
 
-| unop {op: unop} {t t': term}:
-    term.substituted t t' →
-    term.substituted (term.unop op t) (term.unop op t')
+def qfprop.subst_env: env → qfprop → qfprop
+| env.empty P := P
+| (σ[x↦v]) P :=
+    have σ.size < (σ[x ↦ v].size), from lt_of_add_one,
+    qfprop.subst x v (qfprop.subst_env σ P)
 
-| binop {op: binop} {t₁ t₂ t₁' t₂': term}:
-    term.substituted t₁ t₁' →
-    term.substituted t₂ t₂' →
-    term.substituted (term.binop op t₁ t₂) (term.binop op t₁' t₂')
+lemma not_free_of_subst_term {t: term} {x: var} {v: value}: ¬(free_in_term x (term.subst x v t)) :=
+  begin
+    induction t with v' y unop t₁ x_not_free_in_t₁ binop t₂ t₃ x_not_free_in_t₂ x_not_free_in_t₃
+                     t₄ t₅ x_not_free_in_t₄ x_not_free_in_t₅,
+    show ¬free_in_term x (term.subst x v (term.value v')), from (
+      assume x_free_in_v': free_in_term x (term.subst x v (term.value v')),
+      have term.subst x v (term.value v') = v', by unfold term.subst,
+      have free_in_term x v', from this ▸ x_free_in_v',
+      show «false», by cases this
+    ),
+    show ¬free_in_term x (term.subst x v (term.var y)), from (
+      assume x_free_in_y: free_in_term x (term.subst x v (term.var y)),
+      have hite: term.subst x v (term.var y) = (if x = y then v else y), by unfold term.subst,
+      if x_is_y: x = y then
+        have term.subst x v (term.var y) = v, by simp * at *,
+        have free_in_term x v, from this ▸ x_free_in_y,
+        show «false», by cases this
+      else
+        have term.subst x v (term.var y) = y, by simp * at *,
+        have free_in_term x y, from this ▸ x_free_in_y,
+        have x = y, from free_in_term.var.inv this,
+        show «false», from x_is_y this
+    ),
+    show ¬free_in_term x (term.subst x v (term.unop unop t₁)), from (
+      assume x_free_in_unop: free_in_term x (term.subst x v (term.unop unop t₁)),
+      have term.subst x v (term.unop unop t₁) = term.unop unop (term.subst x v t₁), by unfold term.subst,
+      have free_in_term x (term.unop unop (term.subst x v t₁)), from this ▸ x_free_in_unop,
+      have free_in_term x (term.subst x v t₁), from free_in_term.unop.inv this,
+      show «false», from x_not_free_in_t₁ this
+    ),
+    show ¬free_in_term x (term.subst x v (term.binop binop t₂ t₃)), from (
+      assume x_free_in_binop: free_in_term x (term.subst x v (term.binop binop t₂ t₃)),
+      have term.subst x v (term.binop binop t₂ t₃) = term.binop binop (term.subst x v t₂) (term.subst x v t₃),
+      by unfold term.subst,
+      have free_in_term x (term.binop binop (term.subst x v t₂) (term.subst x v t₃)), from this ▸ x_free_in_binop,
+      have free_in_term x (term.subst x v t₂) ∨ free_in_term x (term.subst x v t₃), from free_in_term.binop.inv this,
+      or.elim this (
+        assume : free_in_term x (term.subst x v t₂),
+        show «false», from x_not_free_in_t₂ this
+      ) (
+        assume : free_in_term x (term.subst x v t₃),
+        show «false», from x_not_free_in_t₃ this
+      )
+    ),
+    show ¬free_in_term x (term.subst x v (term.app t₄ t₅)), from (
+      assume x_free_in_app: free_in_term x (term.subst x v (term.app t₄ t₅)),
+      have term.subst x v (term.app t₄ t₅) = term.app (term.subst x v t₄) (term.subst x v t₅),
+      by unfold term.subst,
+      have free_in_term x (term.app (term.subst x v t₄) (term.subst x v t₅)), from this ▸ x_free_in_app,
+      have free_in_term x (term.subst x v t₄) ∨ free_in_term x (term.subst x v t₅), from free_in_term.app.inv this,
+      or.elim this (
+        assume : free_in_term x (term.subst x v t₄),
+        show «false», from x_not_free_in_t₄ this
+      ) (
+        assume : free_in_term x (term.subst x v t₅),
+        show «false», from x_not_free_in_t₅ this
+      )
+    )
+  end
 
-| app {t₁ t₂ t₁' t₂': term}:
-    term.substituted t₁ t₁' →
-    term.substituted t₂ t₂' →
-    term.substituted (term.app t₁ t₂) (term.app t₁' t₂')
-
-inductive spec.substituted (x: var) (v: value): spec → spec → Prop
-
-| term {t t': term} :
-    term.substituted x v t t' →
-    spec.substituted (spec.term t) (spec.term t')
-
-| not {R R': spec} :
-    spec.substituted R R' →
-    spec.substituted (spec.not R) (spec.not R')
-
-| and {R S R' S': spec} :
-    spec.substituted R R' →
-    spec.substituted S S' →
-    spec.substituted (spec.and R S) (spec.and R' S')
-
-| or {R S R' S': spec} :
-    spec.substituted R R' →
-    spec.substituted S S' →
-    spec.substituted (spec.or R S) (spec.or R' S')
-
-| func_same {R S: spec} {t t': term} :
-    term.substituted x v t t' →
-    spec.substituted (spec.func t x R S) (spec.func t' x R S)
-
-| func {y: var} {R S R' S': spec} {t t': term} :
-    (x ≠ y) →
-    term.substituted x v t t' →
-    spec.substituted R R' →
-    spec.substituted S S' →
-    spec.substituted (spec.func t y R S) (spec.func t' y R' S')
-
-inductive spec.substituted_env: env → spec → spec → Prop
-
-| empty {R: spec}:
-    spec.substituted_env env.empty R R
-
-| cons {σ: env} {x: var} {v: value} {R R' R'': spec} :
-    spec.substituted x v R R' →
-    spec.substituted_env σ R' R'' →
-    spec.substituted_env (σ[x↦v]) R R''
-
-inductive qfprop.substituted (x: var) (v: value): qfprop → qfprop → Prop
-
-| term {t t': term} :
-    term.substituted x v t t' →
-    qfprop.substituted (qfprop.term t) (qfprop.term t')
-
-| not {P P': qfprop} :
-    qfprop.substituted P P' →
-    qfprop.substituted (qfprop.not P) (qfprop.not P')
-
-| and {P Q P' Q': qfprop} :
-    qfprop.substituted P P' →
-    qfprop.substituted Q Q' →
-    qfprop.substituted (qfprop.and P Q) (qfprop.and P' Q')
-
-| or {P Q P' Q': qfprop} :
-    qfprop.substituted P P' →
-    qfprop.substituted Q Q' →
-    qfprop.substituted (qfprop.or P Q) (qfprop.or P' Q')
-
-| pre {t₁ t₂ t₁' t₂': term}:
-    term.substituted x v t₁ t₁' →
-    term.substituted x v t₂ t₂' →
-    qfprop.substituted (qfprop.pre t₁ t₂) (qfprop.pre t₁' t₂')
-
-| pre₁ {op: unop} {t t': term} :
-    term.substituted x v t t' →
-    qfprop.substituted (qfprop.pre₁ op t) (qfprop.pre₁ op t')
-
-| pre₂ {op: binop} {t₁ t₂ t₁' t₂': term}:
-    term.substituted x v t₁ t₁' →
-    term.substituted x v t₂ t₂' →
-    qfprop.substituted (qfprop.pre₂ op t₁ t₂) (qfprop.pre₂ op t₁' t₂')
-
-| post {t₁ t₂ t₁' t₂': term}:
-    term.substituted x v t₁ t₁' →
-    term.substituted x v t₂ t₂' →
-    qfprop.substituted (qfprop.post t₁ t₂) (qfprop.post t₁' t₂')
-
-inductive qfprop.substituted_env: env → qfprop → qfprop → Prop
-
-| empty {P: qfprop}:
-    qfprop.substituted_env env.empty P P
-
-| cons {σ: env} {x: var} {v: value} {P P' P'': qfprop} :
-    qfprop.substituted x v P P' →
-    qfprop.substituted_env σ P' P'' →
-    qfprop.substituted_env (σ[x↦v]) P P''
+lemma not_free_of_subst_spec {R: spec} {x: var} {v: value}: ¬ (free_in_prop x (spec.subst x v R).to_prop) :=
+  begin
+    induction R with t S₁ x_not_free_in_S₁ S₂ S₃ x_not_free_in_S₂ x_not_free_in_S₃
+                     S₄ S₅ x_not_free_in_S₄ x_not_free_in_S₅ f fx S₆ S₇ x_not_free_in_S₆ x_not_free_in_S₇,
+    show ¬free_in_prop x (spec.subst x v (spec.term t)).to_prop, from (
+      assume x_free_in_term: free_in_prop x (spec.subst x v (spec.term t)).to_prop,
+      have spec.subst x v (spec.term t) = spec.term (term.subst x v t), by unfold spec.subst,
+      have x_free_in_term': free_in_prop x (spec.term (term.subst x v t)).to_prop, from this ▸ x_free_in_term,
+      have (spec.term (term.subst x v t)).to_prop = prop.term (term.subst x v t), by unfold spec.to_prop,
+      have free_in_prop x (term.subst x v t), from this ▸ x_free_in_term',
+      have free_in_term x (term.subst x v t), from free_in_prop.term.inv this,
+      show «false», from not_free_of_subst_term this
+    ),
+    show ¬free_in_prop x (spec.subst x v S₁.not).to_prop, from (
+      assume x_free_in_not: free_in_prop x (spec.subst x v S₁.not).to_prop,
+      have (spec.subst x v S₁.not = (spec.subst x v S₁).not), by unfold spec.subst,
+      have x_free_in_not': free_in_prop x (spec.subst x v S₁).not.to_prop, from this ▸ x_free_in_not,
+      have (spec.subst x v S₁).not.to_prop = (spec.subst x v S₁).to_prop.not, by unfold spec.to_prop,
+      have free_in_prop x (spec.subst x v S₁).to_prop.not, from this ▸ x_free_in_not',
+      have free_in_prop x (spec.subst x v S₁).to_prop, from free_in_prop.not.inv this,
+      show «false», from x_not_free_in_S₁ this
+    ),
+    show ¬free_in_prop x (spec.subst x v (S₂ & S₃)).to_prop, from (
+      assume x_free_in_and: free_in_prop x (spec.subst x v (S₂ & S₃)).to_prop,
+      have spec.subst x v (spec.and S₂ S₃) = (spec.subst x v S₂ & spec.subst x v S₃), by unfold spec.subst,
+      have x_free_in_and': free_in_prop x (spec.subst x v S₂ & spec.subst x v S₃).to_prop, from this ▸ x_free_in_and,
+      have (spec.and (spec.subst x v S₂) (spec.subst x v S₃)).to_prop
+         = ((spec.subst x v S₂).to_prop & (spec.subst x v S₃).to_prop),
+      by unfold spec.to_prop,
+      have free_in_prop x ((spec.subst x v S₂).to_prop & (spec.subst x v S₃).to_prop), from this ▸ x_free_in_and',
+      have free_in_prop x (spec.subst x v S₂).to_prop ∨ free_in_prop x (spec.subst x v S₃).to_prop,
+      from free_in_prop.and.inv this,
+      or.elim this (
+        assume : free_in_prop x (spec.subst x v S₂).to_prop,
+        show «false», from x_not_free_in_S₂ this
+      ) (
+        assume : free_in_prop x (spec.subst x v S₃).to_prop,
+        show «false», from x_not_free_in_S₃ this
+      )
+    ),
+    show ¬free_in_prop x (spec.subst x v (spec.or S₄ S₅)).to_prop, from (
+      assume x_free_in_or: free_in_prop x (spec.subst x v (spec.or S₄ S₅)).to_prop,
+      have spec.subst x v (spec.or S₄ S₅) = spec.or (spec.subst x v S₄) (spec.subst x v S₅), by unfold spec.subst,
+      have x_free_in_or': free_in_prop x (spec.or (spec.subst x v S₄) (spec.subst x v S₅)).to_prop,
+      from this ▸ x_free_in_or,
+      have (spec.or (spec.subst x v S₄) (spec.subst x v S₅)).to_prop
+         = (prop.or (spec.subst x v S₄).to_prop (spec.subst x v S₅).to_prop),
+      by unfold spec.to_prop,
+      have free_in_prop x (prop.or (spec.subst x v S₄).to_prop (spec.subst x v S₅).to_prop),
+      from this ▸ x_free_in_or',
+      have free_in_prop x (spec.subst x v S₄).to_prop ∨ free_in_prop x (spec.subst x v S₅).to_prop,
+      from free_in_prop.or.inv this,
+      or.elim this (
+        assume : free_in_prop x (spec.subst x v S₄).to_prop,
+        show «false», from x_not_free_in_S₄ this
+      ) (
+        assume : free_in_prop x (spec.subst x v S₅).to_prop,
+        show «false», from x_not_free_in_S₅ this
+      )
+    ),
+    show ¬free_in_prop x (spec.subst x v (spec.func f fx S₆ S₇)).to_prop, from (
+      assume x_free_in_func: free_in_prop x (spec.subst x v (spec.func f fx S₆ S₇)).to_prop,
+      if x_is_fx: x = fx then
+        have h₁: spec.subst x v (spec.func f fx S₆ S₇) = spec.func (term.subst x v f) fx S₆ S₇,
+        by { unfold spec.subst, simp * },
+        let forallp := (prop.implies S₆.to_prop (prop.pre (term.subst x v f) fx)
+                      & prop.implies (S₆.to_prop & prop.post (term.subst x v f) fx) S₇.to_prop) in
+        have h₂: (spec.func (term.subst x v f) fx S₆ S₇).to_prop =
+                 (term.unop unop.isFunc (term.subst x v f) & prop.forallc fx (term.subst x v f) forallp),
+        by unfold spec.to_prop,
+        have free_in_prop x (term.unop unop.isFunc (term.subst x v f) & prop.forallc fx (term.subst x v f) forallp),
+        from h₂ ▸ h₁ ▸ x_free_in_func,
+        have free_in_prop x (term.unop unop.isFunc (term.subst x v f))
+           ∨ free_in_prop x (prop.forallc fx (term.subst x v f) forallp),
+        from free_in_prop.and.inv this,
+        or.elim this (
+          assume : free_in_prop x (term.unop unop.isFunc (term.subst x v f)),
+          have free_in_term x (term.unop unop.isFunc (term.subst x v f)), from free_in_prop.term.inv this,
+          have free_in_term x (term.subst x v f), from free_in_term.unop.inv this,
+          show «false», from not_free_of_subst_term this
+        ) (
+          assume : free_in_prop x (prop.forallc fx (term.subst x v f) forallp),
+          have (x ≠ fx) ∧ (free_in_term x (term.subst x v f) ∨ free_in_prop x forallp),
+          from free_in_prop.forallc.inv this,
+          have ¬ (x = fx), from this.left,
+          show «false», from this x_is_fx
+        )
+      else
+        have h₁: spec.subst x v (spec.func f fx S₆ S₇)
+           = spec.func (term.subst x v f) fx (spec.subst x v S₆) (spec.subst x v S₇),
+        by { unfold spec.subst, simp * },
+        let forallp := (prop.implies (spec.subst x v S₆).to_prop (prop.pre (term.subst x v f) fx)
+                      & prop.implies ((spec.subst x v S₆).to_prop & prop.post (term.subst x v f) fx)
+                                     (spec.subst x v S₇).to_prop) in
+        have h₂: (spec.func (term.subst x v f) fx (spec.subst x v S₆) (spec.subst x v S₇)).to_prop =
+                 (term.unop unop.isFunc (term.subst x v f) & prop.forallc fx (term.subst x v f) forallp),
+        by unfold spec.to_prop,
+        have free_in_prop x (term.unop unop.isFunc (term.subst x v f) & prop.forallc fx (term.subst x v f) forallp),
+        from h₂ ▸ h₁ ▸ x_free_in_func,
+        have free_in_prop x (term.unop unop.isFunc (term.subst x v f))
+           ∨ free_in_prop x (prop.forallc fx (term.subst x v f) forallp),
+        from free_in_prop.and.inv this,
+        or.elim this (
+          assume : free_in_prop x (term.unop unop.isFunc (term.subst x v f)),
+          have free_in_term x (term.unop unop.isFunc (term.subst x v f)), from free_in_prop.term.inv this,
+          have free_in_term x (term.subst x v f), from free_in_term.unop.inv this,
+          show «false», from not_free_of_subst_term this
+        ) (
+          assume : free_in_prop x (prop.forallc fx (term.subst x v f) forallp),
+          have free_in_term x (term.subst x v f) ∨ free_in_prop x forallp,
+          from (free_in_prop.forallc.inv this).right,
+          or.elim this (
+            assume : free_in_term x (term.subst x v f),
+            show «false», from not_free_of_subst_term this
+          ) (
+            assume : free_in_prop x forallp,
+            or.elim (free_in_prop.and.inv this) (
+              assume : free_in_prop x (prop.implies (spec.subst x v S₆).to_prop (prop.pre (term.subst x v f) fx)),
+              or.elim (free_in_prop.implies.inv this) (
+                assume : free_in_prop x (spec.subst x v S₆).to_prop,
+                show «false», from x_not_free_in_S₆ this
+              ) (
+                assume : free_in_prop x (prop.pre (term.subst x v f) fx),
+                or.elim (free_in_prop.pre.inv this) (
+                  assume : free_in_term x (term.subst x v f),
+                  show «false», from not_free_of_subst_term this
+                ) (
+                  assume : free_in_term x fx,
+                  have x = fx, from free_in_term.var.inv this,
+                  show «false», from x_is_fx this
+                )
+              )
+            )
+            (
+              assume : free_in_prop x (prop.implies ((spec.subst x v S₆).to_prop & prop.post (term.subst x v f) fx)
+                                                     (spec.subst x v S₇).to_prop),
+              or.elim (free_in_prop.implies.inv this) (
+                assume : free_in_prop x ((spec.subst x v S₆).to_prop & prop.post (term.subst x v f) fx),
+                or.elim (free_in_prop.and.inv this) (
+                  assume : free_in_prop x (spec.subst x v S₆).to_prop,
+                  show «false», from x_not_free_in_S₆ this
+                ) (
+                  assume : free_in_prop x (prop.post (term.subst x v f) fx),
+                  or.elim (free_in_prop.post.inv this) (
+                    assume : free_in_term x (term.subst x v f),
+                    show «false», from not_free_of_subst_term this
+                  ) (
+                    assume : free_in_term x fx,
+                    have x = fx, from free_in_term.var.inv this,
+                    show «false», from x_is_fx this
+                  )
+                )
+              ) (
+                assume : free_in_prop x (spec.subst x v S₇).to_prop,
+                show «false», from x_not_free_in_S₇ this
+              )
+            )
+          )
+        )
+    )
+  end
 
 -- validity
 
@@ -140,8 +302,48 @@ notation `⊨` p: 100 := valid p
 | mp {q p: qfprop}: ⊨ qfprop.implies p q → ⊨ p → ⊨ q
 
 notation `⊨` p: 100 := valid p
+notation σ `⊨` p: 100 := valid (qfprop.subst_env σ p)
+
+lemma qfprop.subst_env.and {σ: env} {P Q: qfprop}:
+      qfprop.subst_env σ (P & Q) = (qfprop.subst_env σ P & qfprop.subst_env σ Q) :=
+begin
+  induction σ with x v σ' ih,
+  show (qfprop.subst_env env.empty (P & Q) = (qfprop.subst_env env.empty P & qfprop.subst_env env.empty Q)), by begin
+    have h1: (qfprop.subst_env env.empty P = P), by unfold qfprop.subst_env,
+    have h2: (qfprop.subst_env env.empty Q = Q), by unfold qfprop.subst_env,
+    calc
+      qfprop.subst_env env.empty (P & Q) = (P & Q) : by unfold qfprop.subst_env
+                                      ... = (qfprop.subst_env env.empty P & Q) : by rw[h1]
+                                      ... = (qfprop.subst_env env.empty P & qfprop.subst_env env.empty Q) : by rw[h2]
+  end,
+  show (qfprop.subst_env (σ'[x↦v]) (P & Q) = (qfprop.subst_env (σ'[x↦v]) P & qfprop.subst_env (σ'[x↦v]) Q)), by begin
+    have h1: (qfprop.subst x v (qfprop.subst_env σ' P) = qfprop.subst_env (σ'[x↦v]) P), by unfold qfprop.subst_env,
+    calc
+    qfprop.subst_env (σ'[x↦v]) (P & Q) = qfprop.subst x v (qfprop.subst_env σ' (P & Q)) : by unfold qfprop.subst_env
+                                   ... = qfprop.subst x v (qfprop.subst_env σ' P & qfprop.subst_env σ' Q) : by rw[ih]
+                                   ... = (qfprop.subst x v (qfprop.subst_env σ' P) &
+                                          qfprop.subst x v (qfprop.subst_env σ' Q)) : by refl
+                                   ... = (qfprop.subst_env (σ'[x↦v]) P &
+                                          qfprop.subst x v (qfprop.subst_env σ' Q)) : by unfold qfprop.subst_env
+                                   ... = (qfprop.subst_env (σ'[x↦v]) P & qfprop.subst_env (σ'[x↦v]) Q) : by unfold qfprop.subst_env
+  end
+end
+
+lemma valid_env.and {σ: env} {P Q: qfprop}: σ ⊨ P → σ ⊨ Q → σ ⊨ (P & Q) :=
+  assume p_valid: valid (qfprop.subst_env σ P),
+  assume q_valid: valid (qfprop.subst_env σ Q),
+  have qfprop.subst_env σ (P & Q) = (qfprop.subst_env σ P & qfprop.subst_env σ Q), from qfprop.subst_env.and,
+  show σ ⊨ (P & Q), from this.symm ▸ valid.and p_valid q_valid
+
+-- axioms about instantiation
+
+axiom instantiated_p_of_erased_p {σ: env} {P: prop} : σ ⊨ P.erased_p → σ ⊨ P.instantiated_p
+axiom instantiated_n_of_instantiated_p {σ: env} {P: prop} : σ ⊨ P.instantiated_p → σ ⊨ P.instantiated_n
+axiom erased_n_of_instantiated_n {σ: env} {P: prop} : σ ⊨ P.instantiated_n → σ ⊨ P.erased_n
+
+-- notation ⟪ P ⟫
 
 @[reducible]
-def VC(P: prop) := ∀ (σ: env) (P' P'': qfprop), (prop.instantiated P P') → (qfprop.substituted_env σ P' P'') → ⊨ P''
+def VC(P: prop) := ∀ (σ: env), σ ⊨ P.instantiated_p
 
 notation `⟪` P `⟫`: 100 := VC P
